Fixing equality premises; Adding decryption statement in DT6; fixing some lemmas

scripts/DAP_Transaction.thy
@@ -33,7 +33,7 @@ inductive_set daptrans :: "event list set" where
   | DT4: "\<lbrakk> evs4 \<in> daptrans;
             legalUse(Smartphone A); A \<noteq> Server;
             Gets_s (Smartphone A) \<lbrace> Transaction', r', h\<^sub>s \<rbrace> \<in> set evs4;
-            (h\<^sub>s == Hash \<lbrace> Transaction', r' \<rbrace>) \<rbrakk> 
+            h\<^sub>s = Hash \<lbrace> Transaction', r' \<rbrace> \<rbrakk> 
     \<Longrightarrow> Outputs (Smartphone A) A Transaction' # evs4 \<in> daptrans"
 
   | DT5: "\<lbrakk> evs5 \<in> daptrans; legalUse(Smartphone A);
@@ -41,7 +41,7 @@ inductive_set daptrans :: "event list set" where
             Gets A \<lbrace> \<lbrace> Agent A, Number T \<rbrace>, r', h\<^sub>s \<rbrace> \<in> set evs5;
             Inputs A (Smartphone A) \<lbrace> \<lbrace> Agent A, Number T \<rbrace>, r', h\<^sub>s \<rbrace> \<in> set evs5;
             Gets_a A Transaction' \<in> set evs5;
-            Transaction' == \<lbrace> Agent A, Number T \<rbrace> \<rbrakk>
+            Transaction' = \<lbrace> Agent A, Number T \<rbrace> \<rbrakk>
     \<Longrightarrow> Inputs A (Smartphone A) Confirmation # evs5 \<in> daptrans"
 
   | DT6: "\<lbrakk> evs6 \<in> daptrans; legalUse(Smartphone A); A \<noteq> Server;
@@ -49,9 +49,9 @@ inductive_set daptrans :: "event list set" where
             h\<^sub>s == Hash \<lbrace> Transaction', r' \<rbrace>;
             Outputs (Smartphone A) A Transaction' \<in> set evs6; 
             Gets_s (Smartphone A) Confirmation \<in> set evs6;
-            r\<^sub>u \<notin> used evs6 (* This must go away *) \<rbrakk>
+            r' = Crypt (shrK A) (Nonce r) \<rbrakk>
             (* TODO: formalize how r_u is obtained *)
-   \<Longrightarrow> Outputs (Smartphone A) A r\<^sub>u # evs6 \<in> daptrans"
+   \<Longrightarrow> Outputs (Smartphone A) A (Nonce r) # evs6 \<in> daptrans"
 
   | DT7: "\<lbrakk> evs7 \<in> daptrans; A \<noteq> Server;
             Says A Server Transaction \<in> set evs7;
@@ -64,9 +64,7 @@ inductive_set daptrans :: "event list set" where
 
   | DT8: "\<lbrakk> evs8 \<in> daptrans;
             Gets Server Transaction \<in> set evs8;
-            Says Server A \<lbrace>
-              Transaction,
-              Crypt (shrK A) (Nonce r),
+            Says Server A \<lbrace> Transaction, Crypt (shrK A) (Nonce r),
               Hash \<lbrace> Transaction, Crypt (shrK A) (Nonce r) \<rbrace>
             \<rbrace> \<in> set evs8;
             Gets Server r\<^sub>u \<in> set evs8;
@@ -243,14 +241,14 @@ oops
 lemma Outputs_A_Smartphone_4 :
   "\<lbrakk> Outputs P A Transaction' \<in> set evs; evs \<in> daptrans \<rbrakk>
     \<Longrightarrow> legalUse(P) \<and> P = (Smartphone A) \<and>
-        (\<exists> T r' Checksum. (Inputs A (Smartphone A) 
+        (\<exists> T r' Checksum. (Gets_s (Smartphone A) 
           \<lbrace> Transaction', r', Checksum \<rbrace> \<in> set evs))"
 apply (erule rev_mp, erule daptrans.induct)
 apply (auto)
-oops
+done
 
 lemma Outputs_which_Smartphone_4 :
-  "\<lbrakk> Outputs (Smartphone A) A Transaction \<in> set evs; evs \<in> daptrans \<rbrakk>
+  "\<lbrakk> Outputs (Smartphone A) A Transaction' \<in> set evs; evs \<in> daptrans \<rbrakk>
     \<Longrightarrow> \<exists> T r' Checksum. Inputs A (Smartphone A) \<lbrace> \<lbrace>Agent A, Number T\<rbrace>, r', Checksum \<rbrace> \<in> set evs"
 apply (erule rev_mp, erule daptrans.induct)
 apply (simp_all (no_asm_simp))
